Checkpoint.

src/program_logic/crash_weakestpre.v
@@ -5,219 +5,6 @@ From Perennial.program_logic Require Import staged_invariant.
 Set Default Proof Using "Type".
 Import uPred.
 
-Notation "|={ E1 , E2 }_ k => P" :=
-    (|={E1, ∅}=> |={∅, ∅}▷=>^k |={∅, E2}=> P)%I
-      (at level 99, E1, E2 at level 50, k at level 9, P at level 200,
-       format "|={ E1 , E2 }_ k =>  P").
-
-
-Notation "|={ E1 , E2 }_ k =>^ n P" :=
-    (Nat.iter n (λ Q, (|={E1, ∅}=> |={∅, ∅}▷=>^k |={∅, E2}=> Q)) P)%I
-      (at level 99, E1, E2 at level 50, k, n at level 9, P at level 200,
-       format "|={ E1 , E2 }_ k =>^ n  P").
-
-
-Section step_fupdN.
-
-Context {PROP: sbi} {H: BiFUpd PROP} {HAff: BiAffine PROP}.
-
-Lemma step_fupdN_le {E1 E2 : coPset} (n1 n2 : nat) (P: PROP):
-  E2 ⊆ E1 →
-  n1 ≤ n2 → (|={E1,E2}▷=>^n1 P) -∗ |={E1,E2}▷=>^n2 P.
-Proof.
-  intros ?. induction 1 => //=.
-  iIntros. iApply step_fupd_intro; auto. iNext. by iApply IHle.
-Qed.
-
-Lemma step_fupdN_later E1 E2 k (P: PROP):
-  E2 ⊆ E1 →
-  ▷^k P -∗ |={E1,E2}▷=>^k P.
-Proof using HAff.
-  iIntros (Hle).
-  iInduction k as [| k] "IH".
-  - eauto.
-  - iIntros. rewrite Nat_iter_S. iMod (fupd_intro_mask' _ E2) as "Hclo".
-    { set_solver. }
-    iModIntro. iModIntro. iMod "Hclo". iModIntro. by iApply "IH".
-Qed.
-
-Lemma step_fupdN_inner_later E1 E2 k (P: PROP):
-  E2 ⊆ E1 →
-  ▷^k P -∗ |={E1,∅}=> |={∅,∅}▷=>^k |={∅,E2}=> P.
-Proof using HAff.
-  iIntros (Hle).
-  iInduction k as [| k] "IH".
-  - rewrite //=. iIntros "HP".
-    iMod (fupd_intro_mask' _ E2) as "H"; eauto.
-    iApply fupd_intro_mask; eauto; first set_solver.
-  - iIntros. iMod (fupd_intro_mask' _ ∅) as "Hclo".
-    { set_solver. }
-    rewrite Nat_iter_S.
-    iModIntro. iModIntro. iNext. iMod "Hclo". by iApply "IH".
-Qed.
-
-Lemma step_fupdN_inner_fupd E1 E2 k (P: PROP):
-  (|={E1,∅}=> |={∅,∅}▷=>^k |={∅,E2}=> |={E2}=> P) -∗
-  |={E1,∅}=> |={∅,∅}▷=>^k |={∅,E2}=> P.
-Proof.
-  iIntros "H". iMod "H". iApply (step_fupdN_wand with "H").
-  iModIntro. iIntros "H". by iMod "H".
-Qed.
-
-Lemma step_fupdN_inner_plain `{BP: BiPlainly PROP} `{@BiFUpdPlainly PROP H BP}
-      (k: nat) (P: PROP) :
-  Plain P →
-  ((|={⊤, ∅}=> |={∅, ∅}▷=>^k |={∅, ∅}=> P) -∗
-  |={⊤}=> ▷^(S k) P)%I.
-Proof.
-  iIntros (HPlain).
-  iInduction k as [| k] "IH" forall (P HPlain).
-  - rewrite //=. iIntros "H". iApply fupd_plain_mask. do 2 iMod "H".
-    by iModIntro.
-  - iIntros "H".
-    iApply fupd_plain_mask.
-    iMod "H". rewrite -step_fupdN_S_fupd.
-    iMod (step_fupdN_plain with "H") as "H".
-    iModIntro. rewrite -!later_laterN !laterN_later.
-    iNext. iNext. by iMod "H".
-Qed.
-
-Lemma step_fupdN_inner_wand E1 E2 k1 k2 (P Q: PROP):
-  E2 ⊆ E1 →
-  k2 ≤ k1 →
-  (|={E2,∅}=> |={∅,∅}▷=>^k2 |={∅,E2}=> P) -∗
-  (P -∗ Q) -∗
-  |={E1,∅}=> |={∅,∅}▷=>^k1 |={∅,E1}=> Q.
-Proof.
-  iIntros (??) "HP HPQ".
-  iMod (fupd_intro_mask' _ E2) as "Hclo"; auto.
-  iMod "HP". iModIntro.
-  iApply (step_fupdN_le k2 _); auto.
-  iApply (step_fupdN_wand with "HP").
-  iIntros "HP". iMod "HP". iMod "Hclo" as "_".
-  iModIntro. by iApply "HPQ".
-Qed.
-
-Lemma step_fupdN_innerN_wand E1 E2 k1 k2 n1 n2 (P Q: PROP):
-  E2 ⊆ E1 →
-  k2 ≤ k1 →
-  n2 ≤ n1 →
-  (|={E2,E2}_k2=>^n2 P) -∗
-  (P -∗ Q) -∗
-  (|={E1,E1}_k1=>^n1 Q).
-Proof using HAff.
-  iIntros (?? Hle) "HP HPQ".
-  iInduction Hle as [] "IH".
-  {
-    iInduction n2 as [|n2] "IH".
-    { iApply "HPQ". eauto. }
-    rewrite !Nat_iter_S.
-    iApply  (step_fupdN_inner_wand with "HP"); auto.
-    iIntros. iApply ("IH" with "[$] [$]").
-  }
-  rewrite Nat_iter_S.
-  iApply (step_fupdN_inner_later); first auto.
-  iNext. by iApply ("IH" with "[$] [$]").
-Qed.
-
-Lemma step_fupdN_inner_wand' E1 E1' E2 E2' k1 k2 (P Q: PROP):
-  E2 ⊆ E1 →
-  E1' ⊆ E2' →
-  k2 ≤ k1 →
-  (|={E2,∅}=> |={∅,∅}▷=>^k2 |={∅,E2'}=> P) -∗
-  (P -∗ Q) -∗
-  |={E1,∅}=> |={∅,∅}▷=>^k1 |={∅,E1'}=> Q.
-Proof using HAff.
-  iIntros (???) "HP HPQ".
-  iMod (fupd_intro_mask' _ E2) as "Hclo"; auto.
-  iMod "HP". iModIntro.
-  iApply (step_fupdN_le k2 _); auto.
-  iApply (step_fupdN_wand with "HP").
-  iIntros "HP". iMod "HP". iApply fupd_mask_weaken; auto.
-  by iApply "HPQ".
-Qed.
-
-Lemma step_fupdN_innerN_wand' E1 E2 k n (P Q: PROP):
-  (|={E1,E2}_k=>^n P) -∗
-  (P -∗ Q) -∗
-  |={E1,E2}_k=>^n Q.
-Proof using HAff.
-  iIntros "HP HPQ". iInduction n as [| n] "IH".
-  - rewrite //=. by iApply "HPQ".
-  - rewrite //=. iApply (step_fupdN_inner_wand' with "HP"); eauto.
-    iIntros; by iApply ("IH" with "[$] [$]").
-Qed.
-
-Lemma step_fupdN_innerN_S_fupd E1 E2 k n (P: PROP):
-  (|={E1,E2}_k=>^(S n) |={E2}=> P) -∗
-  (|={E1,E2}_k=>^(S n) P).
-Proof using HAff.
-  rewrite !Nat_iter_S_r.
-  iIntros "H". iApply (step_fupdN_innerN_wand' with "H").
-  iApply step_fupdN_inner_fupd.
-Qed.
-
-Lemma step_fupdN_inner_plus E1 E2 k1 k2 (P: PROP):
-  (|={E1,∅}=> |={∅,∅}▷=>^k1 |={∅, E1}=> |={E1,∅}=> |={∅,∅}▷=>^k2 |={∅,E2}=> P)
-  ⊢ (|={E1,∅}=> |={∅,∅}▷=>^(k1 + k2) |={∅,E2}=> P)%I.
-Proof using HAff.
-  rewrite Nat_iter_add.
-  iIntros "H". iMod "H". iModIntro.
-  iApply (step_fupdN_mono with "H"). iIntros "H".
-  destruct k2.
-  * simpl. do 3 iMod "H". eauto.
-  * rewrite Nat_iter_S. iMod "H". iMod "H". eauto.
-Qed.
-
-Lemma step_fupdN_ne E1 E2 n:
-  NonExpansive (λ (P: PROP), |={E1, E2}▷=>^n P)%I.
-Proof.
-  induction n => //=.
-  - apply _.
-  - intros ? P Q ->. eauto.
-Qed.
-
-Lemma step_fupdN_inner_plain' `{BP: BiPlainly PROP} `{@BiFUpdPlainly PROP H BP}
-      (k: nat) (P: PROP) :
-  Plain P →
-  ((|={⊤, ⊤}_k=> P) -∗
-  |={⊤}=> ▷^(S k) P)%I.
-Proof using HAff.
-  iIntros (HPlain).
-  iInduction k as [| k] "IH" forall (P HPlain).
-  - rewrite //=. iIntros "H". do 2 iMod "H". eauto.
-  - iIntros "H".
-    iApply (fupd_plain_mask _ ∅).
-    iMod "H".
-    iDestruct (step_fupdN_wand _ _ _ _ (|={∅}=> P)%I with "H []") as "H".
-    { iIntros "H". iMod "H". iApply fupd_mask_weaken; eauto. }
-    rewrite -step_fupdN_S_fupd.
-    iMod (step_fupdN_plain with "H") as "H".
-    iModIntro. rewrite -!later_laterN !laterN_later.
-    iNext. iNext. by iMod "H".
-Qed.
-
-Lemma step_fupdN_innerN_plain `{BP: BiPlainly PROP} `{@BiFUpdPlainly PROP H BP}
-      (k n: nat) (P: PROP) :
-  Plain P →
-  ((|={⊤, ⊤}_k=>^n P) -∗
-  |={⊤}=> ▷^(n * (S k)) P)%I.
-Proof using HAff.
-  iIntros (HPlain).
-  iInduction n as [| n] "IH" forall (P HPlain).
-  - rewrite //=. eauto.
-  - iIntros "H".
-    rewrite Nat_iter_S.
-    iDestruct (step_fupdN_inner_wand with "H []") as "H";
-      [ reflexivity | reflexivity | |].
-    { iApply "IH"; eauto. }
-    rewrite step_fupdN_inner_fupd.
-    iMod (step_fupdN_inner_plain' with "H") as "H".
-    iModIntro. replace (S n * S k) with (S k + (n * S k)) by lia.
-    rewrite laterN_plus; eauto.
-Qed.
-
-End step_fupdN.
 
 
 (* Define a weakestpre with an explicit crash invariant (i.e. there is a postcondition and a crash condition *)
@@ -236,7 +23,7 @@ Definition wpc_pre `{!irisG Λ Σ} `{crashG Σ} (s : stuckness) (k: nat)
           ([∗ list] i ↦ ef ∈ efs, wpc ⊤ ∅ ef fork_post True) ∗
           NC))))
    end ∧
-   (C -∗ |={E2, ∅}=> |={∅, ∅}▷=>^(S k) |={∅, ∅}=> Φc))%I.
+   (C -∗ |={E1,E1}_(S k)=> |={E2, ∅}=> |={∅, ∅}▷=>^(S k) |={∅, ∅}=> Φc))%I.
 
 
 Local Instance wpc_pre_contractive `{!irisG Λ Σ} `{crashG Σ} s k : Contractive (wpc_pre s k).
@@ -309,7 +96,7 @@ Proof.
   (* FIXME: reflexivity, as being called many times by f_equiv and f_contractive
   is very slow here *)
   do 4 (apply step_fupdN_ne || f_contractive || f_equiv); auto; last first.
-  { repeat (f_contractive || f_equiv). auto. }
+  { f_equiv. f_equiv. apply step_fupdN_ne. f_equiv. eauto. }
   do 30 (apply step_fupdN_ne || f_contractive || f_equiv).
   eapply IH; eauto.
   - intros v. eapply dist_le; eauto.
@@ -330,8 +117,11 @@ Proof.
   iIntros "H". iLöb as "IH" forall (E1 E2 e Φ).
   rewrite wp_unfold wpc_unfold /wp_pre /wpc_pre.
   iSplit; last first.
-  - iMod (fupd_intro_mask' _ ∅) as "Hclo"; first by set_solver+.
-    iIntros "HC". iApply step_fupdN_inner_later; auto.
+  - iIntros "HC".
+    iApply step_fupdN_inner_later; auto.
+    do 2 iNext.
+    iMod (fupd_intro_mask' _ ∅) as "Hclo"; first by set_solver+.
+    iApply step_fupdN_inner_later; auto.
   - destruct (to_val e) as [v|]=>//.
     iIntros (σ1 κ κs n) "Hσ".
     iMod (fupd_intro_mask' _ ∅) as "Hclo"; first by set_solver+.
@@ -398,6 +188,9 @@ Proof.
        { iSplit; first auto. iIntros. iApply step_fupdN_inner_later; auto; try set_solver+. }
   - iDestruct "H" as "(_&H)". iIntros "HC".
     iSpecialize ("H" with "[$]").
+    iApply (step_fupdN_inner_wand with "H"); auto.
+    { lia. }
+    iIntros "H".
     iPoseProof (fupd_mask_frame_r _ _ (E2' ∖ E1') with "H") as "H"; first by set_solver+.
     rewrite -union_difference_L; auto.
     iMod "H". rewrite left_id_L.
@@ -427,6 +220,66 @@ Proof.
     iMod ("H" with "[$]").
     iApply step_fupdN_inner_later; auto.
 Qed.
+
+Lemma wpc_strong_crash_frame s1 s2 k1 k2 E1 E2 e Φ Φc Ψc :
+  s1 ⊑ s2 → k1 ≤ k2 → E1 ⊆ E2 →
+  WPC e @ s1; k1; E1 ; ∅ {{ Φ }} {{ Φc }} -∗
+  (C -∗ |={E2, E2}_(k2 - k1)=> Ψc) -∗
+  WPC e @ s2; k2; E2 ; ∅ {{ Φ }} {{ Φc ∗ Ψc }}.
+Proof.
+  iIntros (?? HE) "H HΦ".
+  iLöb as "IH" forall (e E1 E2 HE Φ Φc Ψc).
+  rewrite !wpc_unfold /wpc_pre.
+  iSplit.
+  - destruct (to_val e) as [v|] eqn:?; eauto.
+    {
+      iDestruct "H" as "(H&_)".
+      iMod (fupd_intro_mask' _ E1) as "Hclo"; first by auto.
+      iMod "H". iMod "Hclo" as "_".
+      iModIntro; eauto.
+    }
+    iIntros (σ1 κ κs n) "Hσ HNC".
+    iMod (fupd_intro_mask' E2 E1) as "Hclo"; first done.
+    iDestruct "H" as "(H&_)".
+    iMod ("H" with "[$] [$]") as "H".
+    iModIntro.
+    iApply (step_fupdN_le (S k1)); eauto.
+    { lia. }
+    iApply (step_fupdN_wand with "H"). iIntros "H".
+    iDestruct "H" as "H". iMod "H" as "(%&H)".
+    iModIntro.
+    iSplit; [by destruct s1, s2|]. iIntros (e2 σ2 efs Hstep).
+    iMod ("H" with "[//]") as "H".
+    iApply (step_fupdN_le (S k1)); eauto.
+    { lia. }
+    iApply (step_fupdN_wand with "H"). iModIntro. iIntros "H".
+    iIntros "!>".
+    iMod "H". iMod "H". iIntros "!>". iNext. iMod "H". iMod "Hclo" as "_". iModIntro.
+    iApply (step_fupdN_le (S k1)); eauto.
+    { lia. }
+    iApply (step_fupdN_inner_wand with "H"); auto.
+    iIntros "(Hσ & H & Hefs & HNC)". iFrame.
+    iSplitR "Hefs".
+    ** iApply ("IH" with "[] H [HΦ]"); auto.
+    ** iApply (big_sepL_impl with "Hefs"); iIntros "!#" (k ef _).
+       iIntros "H". eauto. iApply (wpc_strong_mono with "H"); eauto. 
+       iSplit; eauto. iIntros. iApply step_fupdN_inner_later; auto; try set_solver+.
+  - iDestruct "H" as "(_&H)". iIntros "#HC".
+    iSpecialize ("H" with "[$]").
+    iSpecialize ("HΦ" with "[$]").
+    replace (S k2) with (S k1 + (k2 - k1)) by lia.
+    rewrite Nat_iter_add.
+    iMod (fupd_intro_mask' _ E1) as "Hclo"; first by set_solver.
+    iMod "H". iModIntro.
+    iEval (rewrite step_fupdN_S_fupd).
+    iApply (step_fupdN_wand with "H"). iIntros "H".
+    iMod "H".
+    iMod "Hclo".
+    iApply (step_fupdN_inner_wand with "HΦ"); auto. iIntros "HΦ".
+    iApply (step_fupdN_inner_wand with "H"); eauto; try lia.
+    iIntros; by iFrame.
+Qed.
+
 
 Lemma wpc_frame_l s k E1 E2 e Φ Φc R :
   R ∗ WPC e @ s; k; E1 ; E2 {{ Φ }} {{ Φc }} ⊢ WPC e @ s; k; E1 ; E2 {{ v, R ∗ Φ v }} {{ R ∗ Φc }}.
@@ -462,12 +315,15 @@ Proof.
 Qed.
 
 Lemma wpc_value s k E1 E2 Φ Φc v :
-  (|={E1}=> Φ v) ∧ (|={E2, ∅}=> Φc) ⊢ WPC of_val v @ s; k; E1; E2 {{ Φ }} {{ Φc }}.
+  (|={E1}=> Φ v) ∧ (|={E1}=> |={E2, ∅}=> Φc) ⊢ WPC of_val v @ s; k; E1; E2 {{ Φ }} {{ Φc }}.
 Proof.
   rewrite wpc_unfold /wpc_pre to_of_val. iApply and_mono; auto.
-  iIntros "H". iMod "H".
+  iIntros "H". iIntros "HC".
+  iMod "H". iApply step_fupdN_inner_later; auto.
+  do 2 iNext.
+  iMod "H".
   iMod (fupd_intro_mask' _ ∅) as "Hc"; first by set_solver+.
-  iIntros "HC". iApply step_fupdN_inner_later; auto.
+  iApply step_fupdN_inner_later; auto.
 Qed.
 
 Lemma wpc_value' s k E1 E2 Φ Φc v :
@@ -476,7 +332,7 @@ Proof.
   iIntros "H". iApply wpc_value.
   iSplit.
   - iModIntro. iDestruct "H" as "($&_)".
-  - iDestruct "H" as "(_&H)".
+  - iDestruct "H" as "(_&H)". iModIntro.
     iApply fupd_mask_weaken; first by set_solver+. iFrame.
 Qed.
 
@@ -485,7 +341,7 @@ Lemma wpc_value_inv' s k E1 E2 Φ Φc v :
 Proof. rewrite wpc_unfold /wpc_pre to_of_val. iIntros "(?&_)"; auto. Qed.
 
 Lemma fupd_wpc s k E1 E2 e Φ Φc:
-  (|={E1 ∩ E2}=> WPC e @ s; k; E1 ; E2 {{ Φ }} {{ Φc }}) ⊢ WPC e @ s; k; E1 ; E2 {{ Φ }} {{ Φc }}.
+  (|={E1}=> WPC e @ s; k; E1 ; E2 {{ Φ }} {{ Φc }}) ⊢ WPC e @ s; k; E1 ; E2 {{ Φ }} {{ Φc }}.
 Proof.
   rewrite wpc_unfold /wpc_pre. iIntros "H". iSplit.
   - destruct (to_val e) as [v|] eqn:?.
@@ -504,7 +360,7 @@ Proof. iIntros "H". iApply (wpc_strong_mono' with "H"); rewrite ?difference_diag
 
 Lemma wpc_crash s E1 E2 e k Φ Φc:
   WPC e @ s; k; E1 ; E2 {{ Φ }} {{ Φc }} -∗
-  C -∗ |={E2, ∅}_(S k)=> Φc.
+  C -∗ |={E1, E1}_(S k)=> |={E2, ∅}_(S k)=> Φc.
 Proof.
   iIntros "H".
   rewrite wpc_unfold /wpc_pre.
@@ -525,9 +381,9 @@ Proof.
     - iDestruct "H" as "(_&H)".
       iMod (fupd_mask_mono with "H") as "($&_)"; first by set_solver+.
     - iDestruct "H" as "(H&_)".
+      iIntros "HC". iApply step_fupdN_inner_later; auto. do 2 iNext.
       iMod "H".
       iMod (fupd_intro_mask' _ ∅) as "Hclo"; first by set_solver+.
-      iIntros "HC".
       iModIntro. iApply step_fupdN_later; eauto.
   }
   iSplit.
@@ -557,15 +413,19 @@ Proof.
          iSplit.
          *** iMod (fupd_mask_mono with "H") as "($&_)"; first by set_solver+.
          *** iMod (fupd_mask_mono with "H") as "(_&H)"; first by set_solver+.
+             iIntros "HC".
+             iApply step_fupdN_inner_later; auto. do 2 iNext.
              iMod "H".
              iMod (fupd_intro_mask' _ ∅) as "Hclo'"; first by set_solver+.
-             iIntros "HC". iModIntro. iApply step_fupdN_later; eauto.
+             iModIntro. iApply step_fupdN_later; eauto.
       ** edestruct (atomic _ _ _ _ _ Hstep); congruence.
   }
   iDestruct "H" as "(H&_)".
+  iIntros "HC".
+  iApply step_fupdN_inner_later; auto. do 2 iNext.
   iMod "H".
   iMod (fupd_intro_mask' _ ∅) as "Hclo'"; first by set_solver+.
-  iIntros "HC". iModIntro. iApply step_fupdN_later; auto.
+  iModIntro. iApply step_fupdN_later; auto.
 Qed.
 
 Lemma wpc_bind K `{!LanguageCtx K} s k E1 E2 e Φ Φc :
@@ -642,13 +502,15 @@ Lemma wpc_lift_step_fupd s k E E' Φ Φc e1 :
        WPC e2 @ s; k; E; E' {{ Φ }} {{ Φc }} ∗
        [∗ list] ef ∈ efs, WPC ef @ s; k; ⊤; ∅ {{ fork_post }} {{ True }}))
       ∧ |={∅}=> Φc ∗ |={∅, E'}=> state_interp σ1 (κ ++ κs) n)%I
-  ∧ |={E', ∅}=> Φc)%I
+  ∧ |={E}=> |={E', ∅}=> Φc)%I
  ⊢ WPC e1 @ s; k; E; E' {{ Φ }} {{ Φc }}.
 Proof.
   rewrite wpc_unfold /wpc_pre=>->. iIntros "H".
   iSplit; last first.
   { iIntros. iDestruct "H" as "(_&H)".
-    iMod "H". iMod (fupd_intro_mask' _ ∅); first set_solver+.
+    iMod "H".
+    iApply step_fupdN_inner_later; auto; do 2 iNext.
+    iMod "H".
     iModIntro. iApply step_fupdN_later; auto.
   }
   iDestruct "H" as "(H&_)". iIntros (σ1 κ κs n) "Hσ HNC".
