src/program_logic/staged_invariant.v
@@ -4,6 +4,7 @@ From stdpp Require Export namespaces.
 From iris.base_logic.lib Require Import wsat invariants saved_prop.
 From iris.algebra Require Import gmap.
 From iris.proofmode Require Import tactics.
+From Perennial.program_logic Require Export step_fupd_extra.
 Set Default Proof Using "Type".
 Import uPred.
 
@@ -32,12 +33,12 @@ Definition staged_pending `{stagedG Σ} (γ: gname) : iProp Σ :=
 Definition staged_done `{stagedG Σ} (γ: gname) : iProp Σ :=
   own γ (Cinr (to_agree ())).
 
-Definition staged_inv `{!invG Σ, !crashG Σ, !stagedG Σ} (N: namespace) (γ γ': gname) (Q: iProp Σ) : iProp Σ :=
+Definition staged_inv `{!invG Σ, !crashG Σ, !stagedG Σ} (N: namespace) k E E' (γ γ': gname) (Q: iProp Σ) : iProp Σ :=
   (inv N (∃ γprop_stored γprop_remainder Ps Pr,
              own γ (● Excl' (γprop_stored, γprop_remainder)) ∗
              saved_prop_own γprop_stored Ps ∗
              saved_prop_own γprop_remainder Pr ∗
-             □ (C -∗ Ps -∗ Q ∗ Pr) ∗
+             □ (C -∗ Ps -∗ |={E, E'}_k=> Q ∗ Pr) ∗
              (Ps ∨ (Pr ∗ C ∗ staged_done γ'))))%I.
 
 Definition staged_value `{!stagedG Σ} (N: namespace) (γ: gname) (Q Q': iProp Σ) : iProp Σ :=
@@ -58,16 +59,22 @@ Proof. rewrite /C C_aux.(seal_eq). apply _. Qed.
 Global Instance NC_timeless : Timeless NC.
 Proof. rewrite /NC NC_aux.(seal_eq). apply _. Qed.
 
-Global Instance staged_contractive N γ γ' : Contractive (staged_inv N γ γ').
-Proof. rewrite /staged_inv. solve_contractive. Qed.
+Global Instance staged_contractive N k E E' γ γ' : Contractive (staged_inv N k E E' γ γ').
+Proof.
+  rewrite /staged_inv=> n ?? ?.
+  repeat (apply step_fupdN_ne || f_contractive || f_equiv); eauto.
+Qed.
 
-Global Instance staged_ne N γ γ': NonExpansive (staged_inv N γ γ').
-Proof. apply contractive_ne, _. Qed.
+Global Instance staged_ne N k E E' γ γ': NonExpansive (staged_inv N k E E' γ γ').
+Proof.
+  rewrite /staged_inv=> n ?? ?.
+  repeat (apply step_fupdN_ne || f_contractive || f_equiv); eauto using dist_le.
+Qed.
 
-Global Instance staged_proper N γ γ' : Proper ((⊣⊢) ==> (⊣⊢)) (staged_inv N γ γ').
+Global Instance staged_proper N k E E' γ γ' : Proper ((⊣⊢) ==> (⊣⊢)) (staged_inv N k E E' γ γ').
 Proof. apply ne_proper, _. Qed.
 
-Global Instance staged_persistent N γ γ' P : Persistent (staged_inv N γ γ' P).
+Global Instance staged_persistent N k E E' γ γ' P : Persistent (staged_inv N k E E' γ γ' P).
 Proof. rewrite /staged_inv. apply _. Qed.
 
 Lemma pending_done γ: staged_pending γ -∗ staged_done γ -∗ False.
@@ -85,18 +92,25 @@ Proof.
   done.
 Qed.
 
-Lemma staged_inv_iff N γ γ' P Q : ▷ □ (P ↔ Q) -∗ staged_inv N γ γ' P -∗ staged_inv N γ γ' Q.
+Lemma staged_inv_iff N k E E' γ γ' P Q :
+  ▷ □ (P ↔ Q) -∗
+  staged_inv N k E E' γ γ' P -∗
+  staged_inv N k E E' γ γ' Q.
 Proof.
   iIntros "#HPQ". iApply inv_iff. iNext. iAlways. iSplit.
   - iIntros "H". iDestruct "H" as (?? P0 P0') "(?&?&?&#HP0&Hcase)". iExists _, _, P0, P0'. iFrame.
-    iAlways. iIntros. iDestruct ("HP0" with "[$] [$]") as "(?&?)". iFrame. by iApply "HPQ".
+    iAlways. iIntros. iSpecialize ("HP0" with "[$] [$]"). 
+    iApply (step_fupdN_inner_wand' with "HP0"); eauto.
+    iIntros "(?&$)". by iApply "HPQ".
   - iIntros "H". iDestruct "H" as (?? P0 P0') "(?&?&?&#HP0&Hcase)". iExists _, _, P0, P0'. iFrame.
-    iAlways. iIntros. iDestruct ("HP0" with "[$] [$]") as "(?&?)". iFrame. by iApply "HPQ".
+    iAlways. iIntros. iSpecialize ("HP0" with "[$] [$]").
+    iApply (step_fupdN_inner_wand' with "HP0"); eauto.
+    iIntros "(?&$)". by iApply "HPQ".
 Qed.
 
-Lemma staged_inv_alloc N E P Q Qr:
+Lemma staged_inv_alloc N k E E' P Q Qr:
   ▷ Q ∗ □ (C -∗ Q -∗ P ∗ Qr) ={E}=∗
-  ∃ γ γ', staged_inv N γ γ' P ∗ staged_value N γ Q Qr ∗ staged_pending γ'.
+  ∃ γ γ', staged_inv N k E' E' γ γ' P ∗ staged_value N γ Q Qr ∗ staged_pending γ'.
 Proof.
   iMod (saved_prop_alloc Q) as (γprop) "#Hsaved".
   iMod (saved_prop_alloc Qr) as (γprop') "#Hsaved'".
@@ -104,22 +118,26 @@ Proof.
   { apply auth_both_valid_2; [econstructor | reflexivity]. }
   iMod (own_alloc (Cinl (Excl ()))) as (γ') "H".
   { econstructor. }
-  iIntros "HQP".
-  iMod (inv_alloc N E _ with "[HQP H1]") as "HI"; last first.
+  iIntros "(HQ&#HQP)".
+  iMod (inv_alloc N E _ with "[HQ H1]") as "HI"; last first.
   { iModIntro. iExists γ, γ'. iFrame "H". iSplitL "HI".
     - iApply "HI".
     - iExists γprop, γprop'. iFrame. iFrame "#".
   }
   iNext. iExists γprop, γprop', Q, Qr. iFrame. iFrame "#".
-  iDestruct "HQP" as "(HQ&$)". by iLeft.
+  iAlways. iIntros. iApply step_fupdN_inner_later; auto; iNext.
+  iApply "HQP"; by iFrame.
 Qed.
 
-Lemma staged_inv_open E N γ γ' P Q Qr:
-  ↑N ⊆ E → staged_inv N γ γ' P ∗ staged_value N γ Q Qr
-           ={E,E∖↑N}=∗ (▷ ▷ Q ∗ (∀ Q' Qr', ▷ Q' ∗ □ (C -∗ Q' -∗ P ∗ Qr') ={E∖↑N,E}=∗ staged_value N γ Q' Qr')) ∨
-                       (▷ ▷ Qr ∗ C ∗ |={E∖↑N, E}=> emp).
+Lemma staged_inv_open E N k E1 E2 γ γ' P Q Qr:
+  ↑N ⊆ E →
+  E2 ⊆ E1 →
+  staged_inv N k E1 E2 γ γ' P ∗
+  staged_value N γ Q Qr ={E,E∖↑N}=∗
+  (▷ ▷ Q ∗ (∀ Q' Qr', ▷ Q' ∗ □ (C -∗ Q' -∗ |={E1, E2}_k=> P ∗ Qr') ={E∖↑N,E}=∗ staged_value N γ Q' Qr')) ∨
+  (▷ ▷ Qr ∗ C ∗ |={E∖↑N, E}=> emp).
 Proof.
-  iIntros (?) "(#Hinv&Hval)".
+  iIntros (??) "(#Hinv&Hval)".
   iDestruct "Hval" as (γprop γprop') "(Hγ&#Hsaved&#Hsaved')".
   iInv N as (γprop_alt γprop'_alt Qsaved Qrsaved) "H" "Hclose".
   iDestruct "H" as "(>Hγ'&#Hsaved_alt&#Hsaved'_alt&HQ0&Hcase)".
@@ -158,33 +176,45 @@ Proof.
       { by apply auth_update, option_local_update, exclusive_local_update. }
       iMod ("Hclose" with "[Hγ']").
       * iNext. iExists γprop_new, γprop'_new, _, _. iFrame "#". iFrame.
-        iAlways. eauto.
+        iAlways. iIntros. iApply step_fupdN_inner_later; auto; iNext; by iFrame.
       * eauto.
   }
 Qed.
 
-Lemma staged_inv_weak_open E N γ γ' P:
-  ↑N ⊆ E → (staged_inv N γ γ' P ∗ staged_pending γ' ∗ C ={E}=∗ ▷ P)%I.
+Lemma staged_inv_weak_open E N k E1 γ γ' P:
+  ↑N ⊆ E →
+  E1 ⊆ E ∖ ↑N →
+  staged_inv N k E1 E1 γ γ' P ∗
+  staged_pending γ' ∗
+  C -∗ |={E,E}_(S k)=> P.
 Proof.
-  iIntros (?) "(#Hinv&Hpending&#HC)".
+  iIntros (??) "(#Hinv&Hpending&#HC)".
   iInv N as (γprop_alt γprop'_alt Qsaved Qrsaved) "H" "Hclose".
   iDestruct "H" as "(>Hγ'&#Hsaved_alt&#Hsaved'_alt&#HQ0&Hcase)".
   iDestruct "Hcase" as "[HQ|Hfalse]"; last first.
   { iDestruct "Hfalse" as "(?&?&>H)".
     iDestruct (pending_done with "[$] [$]") as "[]".
   }
-  iAssert (▷ (P ∗ Qrsaved))%I with "[HQ]" as "(HQ&HP)".
-  { iNext. iApply "HQ0"; by iFrame. }
+  iMod (fupd_intro_mask' _ E1) as "Hclo_E"; first auto.
+  iMod (fupd_intro_mask' _ (∅)) as "Hclo_E1"; first by set_solver.
+  iModIntro. rewrite Nat_iter_S. iModIntro. iNext.
+  iMod "Hclo_E1" as "_".
+  iMod ("HQ0" with "[$] [$]") as "H".
+  iApply (step_fupdN_wand with "H"). iIntros "!> H".
+  iMod "H" as "(HP&HQr)".
   iMod (pending_upd_done with "[$]") as "#Hdone".
-  iMod ("Hclose" with "[HP Hγ']").
+  iMod "Hclo_E" as "_".
+  iMod ("Hclose" with "[HQr Hγ']").
   { iNext. iExists _, _, _, _. iFrame "Hγ'". iFrame "#". by iRight. }
-  iModIntro. iNext. eauto.
+  iModIntro. eauto.
 Qed.
 
+(*
 Global Instance into_inv_staged_inv1 N γ P : IntoInv (staged_inv N γ P) N := {}.
 
 Definition staged_inv_exact N Pweak P :=
   (∃ γ, staged_inv N γ Pweak ∗ staged_value N γ P)%I.
+*)
 
 (*
 Global Instance into_acc_inv E N γ Pweak P :
